Std/Data/HashMap/Lemmas.lean
@@ -1,11 +1,16 @@
+/-
+Copyright (c) 2022 Wojciech Nawrocki. All rights reserved.
+Released under Apache 2.0 license as described in the file LICENSE.
+Authors: Wojciech Nawrocki
+-/
 import Std.Data.HashMap.Basic
 import Std.Data.HashMap.WF
 import Std.Data.List.Lemmas
 import Std.Data.List.Perm
 import Std.Data.Array.Lemmas
 
-/-- If there is at most one element with the property `p`, erasing one such element
-is the same as filtering out all of them. -/
+/-- If there is at most one element with the property `p`, erasing one such element is the same
+as filtering out all of them. -/
 theorem List.eraseP_eq_filter_of_unique (l : List α) (p : α → Bool)
     : l.Pairwise (p · → !p ·) → l.eraseP p = l.filter (!p ·) := by
   intro h
@@ -20,15 +25,73 @@ theorem List.eraseP_eq_filter_of_unique (l : List α) (p : α → Bool)
       simp [eraseP, filter, hP, filter_eq_self.mpr this]
     | false => simp [eraseP_cons, filter, hP, ih]
 
+theorem List.find?_eq_some {l : List α} {a : α} {p : α → Bool}
+    : l.find? p = some a → a ∈ l ∧ p a := by
+  induction l with
+  | nil => intro h; cases h
+  | cons x xs ih =>
+    unfold find?
+    cases hP : (p x)
+    . intro h
+      simp [List.mem_cons, ih h]
+    . simp
+      intro hEq
+      simp [← hEq, hP]
+
+/-- If there is at most one element with the property `p`, finding that one element is the same
+as finding any. -/
+theorem List.find?_eq_some_of_unique {l : List α} {a : α} {p : α → Bool}
+    : l.Pairwise (p · → !p ·) → (l.find? p = some a ↔ (a ∈ l ∧ p a)) := by
+  refine fun h => ⟨find?_eq_some, ?_⟩
+  induction l with
+  | nil => simp
+  | cons x xs ih =>
+    intro ⟨hMem, hP⟩
+    cases List.mem_cons.mp hMem with
+    | inl hX => simp [find?, ← hX, hP]
+    | inr hXs =>
+      unfold find?
+      cases hPX : (p x) with
+      | false =>
+        apply ih (List.Pairwise.sublist (List.sublist_cons x xs) h) ⟨hXs, hP⟩
+      | true =>
+        cases hP ▸ (Pairwise_cons.mp h |>.left a hXs hPX)
+
 @[simp]
 theorem List.foldl_cons_fn (l₁ l₂ : List α) :
     l₁.foldl (init := l₂) (fun acc x => x :: acc) = l₁.reverse ++ l₂ := by
   induction l₁ generalizing l₂ <;> simp [*]
 
+@[simp]
+theorem List.foldl_append_fn (l₁ : List α) (l₂ : List β) (f : α → List β) :
+    l₁.foldl (init := l₂) (fun acc x => acc ++ f x) = l₂ ++ l₁.bind f := by
+  induction l₁ generalizing l₂ <;> simp [*]
+
+theorem Array.exists_get_of_mem_data {as : Array α} {a : α}
+    : a ∈ as.data → ∃ (i : Fin as.size), a = as[i] := by
+  rw [← Array.toList_eq, Array.toList]
+  apply Array.foldr_induction
+    (motive := fun _ acc => a ∈ acc → ∃ (i : Fin as.size), a = as[i])
+  case h0 => intro h; cases h
+  case hf =>
+    intro i acc ih h
+    cases List.mem_cons.mp h with
+    | inl h => exact ⟨i, h⟩
+    | inr h => exact ih h
+
 namespace Std.HashMap
 open List
 
 variable [BEq α] [Hashable α] [LawfulHashable α] [PartialEquivBEq α]
+
+-- NOTE(WN): These would ideally be solved by a congruence-closure-for-PERs tactic
+-- See https://leanprover.zulipchat.com/#narrow/stream/270676-lean4/topic/Rewriting.20congruent.20relations
+private theorem beq_nonsense_1 {a b c : α} : a != b → a == c → b != c :=
+  fun h₁ h₂ => Bool.bne_iff_not_beq.mpr fun h₃ =>
+    Bool.bne_iff_not_beq.mp h₁ (PartialEquivBEq.trans h₂ (PartialEquivBEq.symm h₃))
+
+private theorem beq_nonsense_2 {a b c : α} : a == b → b == c → ¬(c != a) :=
+  fun h₁ h₂ h₃ => Bool.bne_iff_not_beq.mp (bne_symm h₃) (PartialEquivBEq.trans h₁ h₂)
 
 /-- It is a bit easier to reason about `foldl (append)` than `foldl (foldl)`, so we use this
 (less efficient) variant of `toList` as the mathematical model. -/
@@ -49,7 +112,14 @@ theorem toList_eq_reverse_toListModel (m : HashMap α β) : m.toList = m.toListM
     intro l₂
     simp only [List.foldl, ← List.reverse_append, ih]
 
-/-- The map does not store duplicate (`beq`) keys. -/
+/-- The contents of any given bucket are pairwise `bne`. -/
+theorem Pairwise_bne_bucket (m : HashMap α β) (i : Fin m.val.buckets.val.size) :
+  Pairwise (·.1 != ·.1) m.val.buckets.val[i].toList := by
+  have hWF := Imp.WF_iff.mp m.property |>.right
+  have := hWF.distinct m.val.buckets.val[i] (Array.getElem_mem_data _ _)
+  exact List.Pairwise.imp Bool.bne_iff_not_beq.mpr this
+
+/-- The map does not store duplicate (by `beq`) keys. -/
 theorem Pairwise_bne_toListModel (m : HashMap α β) : m.toListModel.Pairwise (·.1 != ·.1) := by
   unfold toListModel
   refine Array.foldl_induction
@@ -65,10 +135,7 @@ theorem Pairwise_bne_toListModel (m : HashMap α β) : m.toListModel.Pairwise (�
     have hWF := Imp.WF_iff.mp m.property |>.right
     intro i acc h
     refine ⟨List.pairwise_append.mpr ⟨h.left, ?bkt, ?accbkt⟩, ?accbkts⟩
-    case bkt =>
-      -- Main proof 1: the contents of any given bucket are pairwise bne
-      have := hWF.distinct m.val.buckets.val[i] (Array.getElem_mem_data _ _)
-      exact List.Pairwise.imp Bool.not_eq_true_iff_ne_true.mpr this
+    case bkt => apply Pairwise_bne_bucket
     case accbkt =>
       intro a hA b hB
       exact h.right i.val (Nat.le_refl _) i.isLt a hA b hB
@@ -78,7 +145,7 @@ theorem Pairwise_bne_toListModel (m : HashMap α β) : m.toListModel.Pairwise (�
       case inl hP => exact h.right j (Nat.le_of_succ_le hGe) hLt p hP r hR
       case inr hP =>
         -- Main proof 2: distinct buckets store bne keys
-        refine Bool.not_eq_true_iff_ne_true.mpr fun h => ?_
+        refine Bool.bne_iff_not_beq.mpr fun h => ?_
         have hHashEq := LawfulHashable.hash_eq h
         have hGt := Nat.lt_of_succ_le hGe
         have hHashP := hWF.hash_self i (Nat.lt_trans hGt hLt) _ hP
@@ -94,9 +161,53 @@ theorem toListModel_eraseP_eq_toListModel_filter (m : HashMap α β)
   apply List.eraseP_eq_filter_of_unique
   apply List.Pairwise.imp ?_ (Pairwise_bne_toListModel _)
   intro (a₁, _) (a₂, _) hA₁Bne hA₁Beq
-  rw [Bool.not_eq_true_iff_ne_true]
-  intro hA₂Beq
-  exact Bool.not_bne_of_beq (PartialEquivBEq.trans hA₁Beq (PartialEquivBEq.symm hA₂Beq)) hA₁Bne
+  rw [Bool.not_eq_true_iff_ne_true, ← Bool.bne_iff_not_beq]
+  exact beq_nonsense_1 hA₁Bne hA₁Beq
+
+theorem mem_toListModel_iff_mem_bucket (m : HashMap α β) (a : α) (b : β)
+    : haveI := Imp.mkIdx m.val.buckets.2 a
+      (a, b) ∈ m.toListModel ↔ (a, b) ∈ (m.val.buckets.val[this.1]'this.2).toList := by
+  have : (a, b) ∈ m.toListModel ↔ ∃ bkt ∈ m.val.buckets.val.data, (a, b) ∈ bkt.toList := by
+    simp [toListModel, Array.foldl_eq_foldl_data, List.foldl_append_fn, List.nil_append,
+      List.mem_bind]
+  rw [this]
+  clear this
+  apply Iff.intro
+  . intro ⟨bkt, hBkt, hMem⟩
+    have ⟨i, hGetI⟩ := Array.exists_get_of_mem_data hBkt
+    simp only [getElem_fin] at hGetI
+    suffices (Imp.mkIdx m.val.buckets.2 a).val.toNat = i by
+      simp [Array.ugetElem_eq_getElem, this, ← hGetI, hMem]
+    unfold Imp.mkIdx
+    dsimp
+    exact Imp.WF_iff.mp m.property |>.right |>.hash_self i.val i.isLt (a, b) (hGetI ▸ hMem)
+  . intro h
+    refine ⟨_, Array.getElem_mem_data _ _, h⟩
+
+theorem findEntry?_eq (m : HashMap α β) (a : α)
+    : m.findEntry? a = m.toListModel.find? (·.1 == a) := by
+  have hPairwiseM : Pairwise (fun p q => p.1 == a → q.1 != a) m.toListModel :=
+    Pairwise.imp (fun p q => beq_nonsense_1 p q) (Pairwise_bne_toListModel m)
+  have hPairwiseBkt :
+      haveI := Imp.mkIdx m.val.buckets.property a
+      Pairwise (fun p q => p.1 == a → q.1 != a) (m.val.buckets.val[this.1]'this.2).toList := by
+    sorry
+  apply Option.ext
+  intro (a', b)
+  simp only [Option.mem_def, findEntry?, Imp.findEntry?, AssocList.findEntry?_eq,
+    List.find?_eq_some_of_unique hPairwiseM, List.find?_eq_some_of_unique hPairwiseBkt,
+    and_congr_left_iff]
+  intro hBeq
+  have : hash a' = hash a := LawfulHashable.hash_eq hBeq
+  simp [mem_toListModel_iff_mem_bucket, Imp.mkIdx, this]
+
+theorem findEntry?_eq_some (m : HashMap α β) (a : α) (b : β)
+    : m.findEntry? a = some (a, b) ↔ (∃ a', a == a' ∧ (a', b) ∈ m.toListModel) := by
+  sorry
+
+theorem find?_eq (m : HashMap α β) (a : α)
+    : m.find? a = (m.findEntry? a).map (·.2) := by
+  sorry
 
 theorem toListModel_insert_perm_cons_eraseP (m : HashMap α β) (a : α) (b : β)
     : (m.insert a b).toListModel ~ (a, b) :: m.toListModel.eraseP (·.1 == a) :=
@@ -113,19 +224,6 @@ theorem toListModel_erase_perm_eraseP (m : HashMap α β) (a : α)
 theorem toListModel_erase (m : HashMap α β) (a : α)
     : (m.erase a).toListModel ~ m.toListModel.filter (·.1 != a) :=
   toListModel_eraseP_eq_toListModel_filter m ▸ toListModel_erase_perm_eraseP m a
-
-theorem findEntry?_eq (m : HashMap α β) (a : α)
-    : m.findEntry? a = m.toListModel.find? (·.1 == a) := by
-  unfold findEntry? Imp.findEntry?
-  conv => simp_match; simp_match
-  sorry
-
-theorem find?_of_toListModel_contains (m : HashMap α β) (a : α) (b : β)
-    : (∃ a', a == a' ∧ (a', b) ∈ m.toListModel) ↔ m.find? a = some b := by
-  unfold HashMap.toListModel HashMap.find? Imp.find?
-  -- have H : (∃ a', a == a' ∧ (a', b) ∈ m.toListModel)
-  --     ↔ (∃ a', ∃ bkt, (i : Fin m.val.buckets.val.size) → bkt = m.val.buckets.val[i] → (a',b) ∈ bkt) := sorry
-  sorry
 
 theorem find?_of_toListModel_not_contains (m : HashMap α β) (a : α)
     : (∀ a' (b : β), a == a' → (a', b) ∉ m.toListModel) ↔ m.find? a = none := by
@@ -153,8 +251,8 @@ theorem find?_insert_of_ne (m : HashMap α β) (a a' : α) (b : β)
   apply Option.ext
   intro b'
   show find? (insert m a b) a' = some b' ↔ find? m a' = some b'
-  simp only [← find?_of_toListModel_contains, List.Perm.mem_iff (toListModel_insert m a b), List.mem_cons,
-    List.mem_filter, Prod.mk.injEq]
+  simp only [← find?_of_toListModel_contains, List.Perm.mem_iff (toListModel_insert m a b),
+    List.mem_cons, List.mem_filter, Prod.mk.injEq]
   apply Iff.intro
   . intro ⟨a'', hA', h⟩
     cases h with
@@ -175,7 +273,7 @@ theorem find?_erase (m : HashMap α β) (a a')
   apply (find?_of_toListModel_not_contains _ _).mp
   intro a₂ b hA₂ hMem
   rw [List.Perm.mem_iff (toListModel_erase m a)] at hMem
-  refine Bool.not_bne_of_beq (PartialEquivBEq.symm <| PartialEquivBEq.trans hEq hA₂) ?_
-  exact List.mem_filter.mp hMem |>.right
+  have := List.mem_filter.mp hMem |>.right
+  exact beq_nonsense_2 hEq hA₂ this
 
 end Std.HashMap
